src/Init/Prelude.lean
@@ -3421,23 +3421,26 @@ instance : DecidableEq String := String.decEq
 A byte position in a `String`, according to its UTF-8 encoding.
 
 Character positions (counting the Unicode code points rather than bytes) are represented by plain
-`Nat`s. Indexing a `String` by a `String.Pos` takes constant time, while character positions need to
+`Nat`s. Indexing a `String` by a `String.Pos.Raw` takes constant time, while character positions need to
 be translated internally to byte positions, which takes linear time.
 
 A byte position `p` is *valid* for a string `s` if `0 ≤ p ≤ s.endPos` and `p` lies on a UTF-8
-character boundary.
+character boundary, see `String.Pos.IsValid`.
+
+There is another type, `String.ValidPos`, which bundles the validity predicate. Using `String.ValidPos`
+instead of `String.Pos.Raw` is recommended because it will lead to less error handling and fewer edge cases.
 -/
-structure String.Pos where
-  /-- Get the underlying byte index of a `String.Pos` -/
+structure String.Pos.Raw where
+  /-- Get the underlying byte index of a `String.Pos.Raw` -/
   byteIdx : Nat := 0
 
-instance : Inhabited String.Pos where
+instance : Inhabited String.Pos.Raw where
   default := {}
 
-instance : DecidableEq String.Pos :=
+instance : DecidableEq String.Pos.Raw :=
   fun ⟨a⟩ ⟨b⟩ => match decEq a b with
     | isTrue h => isTrue (h ▸ rfl)
-    | isFalse h => isFalse (fun he => String.Pos.noConfusion he fun he => absurd he h)
+    | isFalse h => isFalse (fun he => String.Pos.Raw.noConfusion he fun he => absurd he h)
 
 /--
 A region or slice of some underlying string.
@@ -3456,9 +3459,9 @@ structure Substring where
   /-- The underlying string. -/
   str      : String
   /-- The byte position of the start of the string slice. -/
-  startPos : String.Pos
+  startPos : String.Pos.Raw
   /-- The byte position of the end of the string slice. -/
-  stopPos  : String.Pos
+  stopPos  : String.Pos.Raw
 
 instance : Inhabited Substring where
   default := ⟨"", {}, {}⟩
@@ -3484,7 +3487,7 @@ A UTF-8 byte position that points at the end of a string, just after the last ch
 * `"abc".endPos = ⟨3⟩`
 * `"L∃∀N".endPos = ⟨8⟩`
 -/
-@[inline] def String.endPos (s : String) : String.Pos where
+@[inline] def String.endPos (s : String) : String.Pos.Raw where
   byteIdx := utf8ByteSize s
 
 /--
@@ -4698,7 +4701,7 @@ inductive SourceInfo where
   The `leading` whitespace is inferred after parsing by `Syntax.updateLeading`. This is because the
   “preceding token” is not well-defined during parsing, especially in the presence of backtracking.
   -/
-  | original (leading : Substring) (pos : String.Pos) (trailing : Substring) (endPos : String.Pos)
+  | original (leading : Substring) (pos : String.Pos.Raw) (trailing : Substring) (endPos : String.Pos.Raw)
   /--
   Synthetic syntax is syntax that was produced by a metaprogram or by Lean itself (e.g. by a
   quotation). Synthetic syntax is annotated with a source span from the original syntax, which
@@ -4722,7 +4725,7 @@ inductive SourceInfo where
   ```
   In these cases, if the user hovers over `h` they will see information about both binding sites.
   -/
-  | synthetic (pos : String.Pos) (endPos : String.Pos) (canonical := false)
+  | synthetic (pos : String.Pos.Raw) (endPos : String.Pos.Raw) (canonical := false)
   /-- A synthesized token without position information. -/
   | protected none
 
@@ -4735,7 +4738,7 @@ Gets the position information from a `SourceInfo`, if available.
 If `canonicalOnly` is true, then `.synthetic` syntax with `canonical := false`
 will also return `none`.
 -/
-def getPos? (info : SourceInfo) (canonicalOnly := false) : Option String.Pos :=
+def getPos? (info : SourceInfo) (canonicalOnly := false) : Option String.Pos.Raw :=
   match info, canonicalOnly with
   | original (pos := pos) ..,  _
   | synthetic (pos := pos) (canonical := true) .., _
@@ -4747,7 +4750,7 @@ Gets the end position information from a `SourceInfo`, if available.
 If `canonicalOnly` is true, then `.synthetic` syntax with `canonical := false`
 will also return `none`.
 -/
-def getTailPos? (info : SourceInfo) (canonicalOnly := false) : Option String.Pos :=
+def getTailPos? (info : SourceInfo) (canonicalOnly := false) : Option String.Pos.Raw :=
   match info, canonicalOnly with
   | original (endPos := endPos) ..,  _
   | synthetic (endPos := endPos) (canonical := true) .., _
@@ -4767,7 +4770,7 @@ Gets the end position information of the trailing whitespace of a `SourceInfo`, 
 If `canonicalOnly` is true, then `.synthetic` syntax with `canonical := false`
 will also return `none`.
 -/
-def getTrailingTailPos? (info : SourceInfo) (canonicalOnly := false) : Option String.Pos :=
+def getTrailingTailPos? (info : SourceInfo) (canonicalOnly := false) : Option String.Pos.Raw :=
   match info.getTrailing? with
   | some trailing => some trailing.stopPos
   | none          => info.getTailPos? canonicalOnly
@@ -5114,7 +5117,7 @@ Get the starting position of the syntax, if possible.
 If `canonicalOnly` is true, non-canonical `synthetic` nodes are treated as not carrying
 position information.
 -/
-def getPos? (stx : Syntax) (canonicalOnly := false) : Option String.Pos :=
+def getPos? (stx : Syntax) (canonicalOnly := false) : Option String.Pos.Raw :=
   stx.getHeadInfo.getPos? canonicalOnly
 
 /--
@@ -5122,7 +5125,7 @@ Get the ending position of the syntax, if possible.
 If `canonicalOnly` is true, non-canonical `synthetic` nodes are treated as not carrying
 position information.
 -/
-partial def getTailPos? (stx : Syntax) (canonicalOnly := false) : Option String.Pos :=
+partial def getTailPos? (stx : Syntax) (canonicalOnly := false) : Option String.Pos.Raw :=
   match stx, canonicalOnly with
   | atom (SourceInfo.original (endPos := pos) ..) .., _
   | atom (SourceInfo.synthetic (endPos := pos) (canonical := true) ..) _, _
@@ -5134,7 +5137,7 @@ partial def getTailPos? (stx : Syntax) (canonicalOnly := false) : Option String.
   | node (SourceInfo.synthetic (endPos := pos) (canonical := true) ..) .., _
   | node (SourceInfo.synthetic (endPos := pos) ..) .., false => some pos
   | node _ _ args, _ =>
-    let rec loop (i : Nat) : Option String.Pos :=
+    let rec loop (i : Nat) : Option String.Pos.Raw :=
       match decide (LT.lt i args.size) with
       | true => match getTailPos? (args.get!Internal ((args.size.sub i).sub 1)) canonicalOnly with
          | some info => some info
