src/Init/SizeOf.lean
@@ -87,7 +87,7 @@ deriving instance SizeOf for List
 deriving instance SizeOf for Array
 deriving instance SizeOf for ByteArray
 deriving instance SizeOf for String
-deriving instance SizeOf for String.Pos
+deriving instance SizeOf for String.Pos.Raw
 deriving instance SizeOf for Substring
 deriving instance SizeOf for Except
 deriving instance SizeOf for EStateM.Result
